src/parser/FStarC.Parser.AST.Util.fst
@@ -196,6 +196,8 @@ let lookup_extension_parser (ext:string) : ML _ =
     else None
   | r -> r
 
+let mk_extension_lang_parser f = { parse_decls = f }
+
 let as_open_namespaces_and_abbrevs (ls:list decl)
 : ML open_namespaces_and_abbreviations
 = List.fold_right
